A try to define behavior

IOHist.fst
@@ -58,21 +58,99 @@ let rec iohist_interpretation #a
       iohist_interpretation (fnc res) (event :: past_events) (gen_post p event)))
   end
 
+type set_of_traces = events_trace -> Type0
 
-let rec fin_prefs #a
-  (m : io a) 
-  (past_events : events_trace) 
-  (traces : list events_trace) : Type0 = 
+val include_in : events_trace -> (set_of_traces) -> Type0
+let include_in t set = set t
+
+val subset : set_of_traces -> set_of_traces -> Type0
+let subset s1 s2 = forall t. s1 t ==>  s2 t
+
+let rec behavior #a
+  (m : io a) : set_of_traces =
   match m with
-  | Return x -> past_events `List.memP` traces
-  | Throw err -> past_events `List.memP` traces
+  | Return x -> fun t -> t == []
+  | Throw err -> fun t -> t == []
   | Cont t -> begin
     match t with
-    | Call cmd args fnc -> (forall res. (
-      FStar.WellFounded.axiom1 fnc res;
-      let event : io_event = convert_call_to_event cmd args res in
-      fin_prefs (fnc res) (event :: past_events) traces))
+    | Call cmd args fnc -> (fun t' -> 
+      (exists res t. (
+         FStar.WellFounded.axiom1 fnc res;
+         ((include_in t (behavior (fnc res))) /\
+         t' == ((convert_call_to_event cmd args res)::t)))))
   end
+
+let l : events_trace = []
+#set-options "--max_fuel 20 --max_ifuel 20"
+let _ = assert (include_in [EOpenfile "asdf" (Inl 7)] (behavior (Cont (Call Openfile "asdf" (fun x -> Return x))))) by (
+  unfold_def (`behavior);
+  unfold_def (`include_in);
+  unfold_def (`convert_call_to_event);
+  witness (`(Inl 7));
+  witness (`l);
+  dump "h")
+
+let code1 : io (res Close) = 
+  io_bind _ _
+    (io_openfile "asdf")
+    io_close
+
+
+exception OneExc
+let _ = assert (include_in [EOpenfile "asdf" (Inr OneExc)] (behavior code1)) by (
+  unfold_def (`code1);
+  unfold_def (`behavior);
+  unfold_def (`include_in);
+  unfold_def (`convert_call_to_event);
+  witness (`(Inr OneExc));
+  witness (`l);
+  dump "h")
+
+
+// let _ = assert (include_in [EOpenfile "asdf" (Inl 7); EClose 8 (Inl ())] (behavior code1)) by (
+//   unfold_def (`code1);
+//   unfold_def (`behavior);
+//   unfold_def (`include_in);
+//   unfold_def (`convert_call_to_event);
+//   witness (`(Inl 7));
+//   witness (`([EClose 8 (Inl ())]));
+//   // witness (`(Inl ()));
+//   // witness (`l);
+//   dump "h")
+
+let rec behavior' #a
+  (m : io a)
+  (p : set_of_traces) : Type0 =
+  match m with
+  | Return x -> p []
+  | Throw err ->  p []
+  | Cont t -> begin
+    match t with
+    | Call cmd args fnc -> exists res. (
+         FStar.WellFounded.axiom1 fnc res;
+      (behavior' (fnc res) (fun t' -> p ((convert_call_to_event cmd args res)::t'))))
+      // (exists res t. (
+      //    FStar.WellFounded.axiom1 fnc res;
+      //    (p ((convert_call_to_event cmd args res)::t))
+      //         /\ (include_in t (behavior' (fnc res))))))
+  end
+
+#set-options "--max_fuel 20 --max_ifuel 20"
+let _ = assert (behavior' (Cont (Call Openfile "asdf" (fun x -> Return x))) (fun trace -> trace == [EOpenfile "asdf" (Inl 7)])) by (
+  unfold_def (`behavior');
+  unfold_def (`convert_call_to_event);
+  witness (`(Inl 7));
+  explode ();
+  dump "h")
+
+let _ = assert (behavior' code1 (fun trace -> trace == [EOpenfile "asdf" (Inr OneExc)])) by (
+  unfold_def (`code1);
+  unfold_def (`behavior');
+  unfold_def (`convert_call_to_event);
+  witness (`(Inr OneExc));
+  witness (`l);
+  compute ();
+  dump "h")
 
 (* total *)
 (* reifiable *)
