IOStHist.fst
@@ -1,20 +1,19 @@
 module IOStHist
 
 open FStar.Tactics
-
-open Common
+open ExtraTactics
 open FStar.Exn
 open FStar.ST
-include IO.Free
-include IOHist
-include ExtraTactics
 
-// Extraction hack
+open Common
+open IO.Free
+open IOHist
+
 val hh : ref events_trace
 let hh = ST.alloc []
 
 let get_history () = !hh
-let update_history (event) =
+let update_history (event) = 
   hh := event :: !hh
   
 // UTILS
@@ -31,7 +30,11 @@ let rec is_open (fd:file_descr) (past_events: events_trace) :
 
 type action_type = (cmd : io_cmds) & (args cmd)
 
-// UNREFINED COMPUTATION MONAD
+unfold let convert_event_to_action (event:io_event) : action_type = 
+  match event with
+  | EOpenfile args _ -> (| Openfile, args |)
+  | ERead args _ -> (| Read, args |)
+  | EClose args _ -> (| Close, args |)
 
 type iost a = events_trace -> io (events_trace * a)
 
@@ -40,113 +43,74 @@ let iost_return (a:Type) (x:a) : iost a = fun s -> io_return (events_trace * a) 
   
 unfold
 let iost_throw (a:Type) (x:exn) : iost a = fun s -> io_throw (events_trace * a) x
-  
+
 unfold
 let iost_bind (a:Type) (b:Type) (l : iost a) (k : a -> iost b) : iost b =
-  fun s -> io_bind (events_trace * a)
-                (events_trace * b)
-                (l s)
-                (fun (s', x) -> k x s')
-
-// SPEC MONAD
+  fun s -> io_bind (events_trace * a) 
+                (events_trace * b) 
+                (l s) 
+                (fun (s', x) -> k x s') 
 
 let iosthist_post a = maybe (s1:events_trace * a) -> (le:events_trace) -> Type0  // local_events (from old to new)
-let iosthist_wpty a = (s0:events_trace) -> iosthist_post a -> Type0
+let iosthist_wpty a = (s0:events_trace) -> iosthist_post a -> Type0  
 
 unfold let iosthist_return_wp (a:Type) (x:a) : iosthist_wpty a =
   fun s0 p -> p (Inl (s0, x)) []
 
 unfold
-let compute_post (a b:Type) (kw : a -> iosthist_wpty b) (p:iosthist_post b)
-  : iosthist_post a =
-      (fun result local_events ->
+let iosthist_bind_wp (_ : range) (a:Type) (b:Type) (w : iosthist_wpty a) (kw : a -> iosthist_wpty b) : iosthist_wpty b =
+  fun s0 p -> 
+    w s0 
+      (fun result local_events -> 
         match result with
         | Inl v -> let (s1, r) = v in
             kw r s1
-            (fun r' local_events' ->
+            (fun r' local_events' -> 
                 p r' (local_events @ local_events'))
         | Inr err -> p (Inr err) local_events)
 
-unfold
-let iosthist_bind_wp (a b:Type) (w : iosthist_wpty a) (kw : a -> iosthist_wpty b) : iosthist_wpty b =
-  fun s0 p -> w s0 (compute_post a b kw p)
-
-// THETA
-
 let iosthist_interpretation #a (m : iost a) (s0 : events_trace) (p : iosthist_post a) : Type0 =
-  iohist_interpretation (m s0) s0 (fun r le -> p r le)
+  iohist_interpretation (m s0) s0 (fun r le -> p r le) 
 
-// REFINED COMPUTATION MONAD (repr)
-let irepr (a:Type) (wp:iosthist_wpty a) =
-  post:iosthist_post a -> h:events_trace ->
-    Pure (io (events_trace * a))
-      (requires (wp h post))
-      (ensures (fun (t:io (events_trace * a)) -> iohist_interpretation t h post))
-
-// let irepr (a:Type) (wp:iosthist_wpty a) =
-//   h:events_trace ->
-//     PURE (io (events_trace * a))
-//       (fun (purepost:io (events_trace * a) -> Type0) ->
-//         forall (post:iosthist_post a).
-//         wp h post /\
-//         (forall (t:io (events_trace * a)). (iohist_interpretation t h post) ==> purepost t))
-
-let ireturn (a : Type) (x : a) : irepr a (iosthist_return_wp a x) =
-  fun _ s0 -> io_return (events_trace * a) (s0, x)
-
-let w = iosthist_wpty
-
-val w_ord (#a : Type) : w a -> w a -> Type0
-let w_ord wp1 wp2 = forall h p. wp1 h p ==> wp2 h p
-
-let ibind (a b : Type) (wp_v : w a) (wp_f: a -> w b) (v : irepr a wp_v)
-  (f : (x:a -> irepr b (wp_f x))) : irepr b (iosthist_bind_wp _ _ wp_v wp_f) =
-  fun p s0 -> 
-    let t = (io_bind (events_trace * a) (events_trace * b)
-        (v (compute_post a b wp_f p) s0)
-        (fun (s1, x) ->
-          assume (wp_f x s1 p);
-           f x p s1)) in
-    assume (iohist_interpretation t s0 p);
-    t
-
-let isubcomp (a:Type) (wp1 wp2: w a) (f : irepr a wp1) :
-  Pure (irepr a wp2) (requires w_ord wp2 wp1) (ensures fun _ -> True) = f
-
-let wp_if_then_else (#a:Type) (wp1 wp2:w a) (b:bool) : w a =
-  fun h p -> (b ==> wp1 h p) /\ ((~b) ==> wp2 h p)
-
-let i_if_then_else (a : Type) (wp1 wp2 : w a) (f : irepr a wp1) (g : irepr a wp2) (b : bool) : Type =
-  irepr a (wp_if_then_else wp1 wp2 b)
-
-/// IOST is the IO monad but a state passing history (materialize past_events).
+// IOST is the IO monad but a state passing history (materialize past_events).
 total
 reifiable
 reflectable
-layered_effect {
-  IOStHistwp : a:Type -> wp : iosthist_wpty a -> Effect
-  with
-       repr       = irepr
-     ; return     = ireturn
-     ; bind       = ibind
+new_effect {
+  IOStHistwp : a:Type -> Effect
+  with 
+       repr       = iost
+     ; return     = iost_return
+     ; bind       = iost_bind
 
-     ; subcomp      = isubcomp
-     ; if_then_else = i_if_then_else
+     ; wp_type    = iosthist_wpty
+     ; return_wp  = iosthist_return_wp
+     ; bind_wp    = iosthist_bind_wp
+
+     ; interp     = iosthist_interpretation
 }
 
 
-let lift_pure_iosthistwp (a:Type) (wp:pure_wp a) (f:(eqtype_as_type unit -> PURE a wp)) :
-  Pure (irepr a (fun s0 p -> wp (fun r -> p (Inl (s0, r)) []))) (requires True)
-                    (ensures (fun _ -> True))
-  = fun p s0 -> let r = elim_pure f (fun r -> p (Inl (s0, r)) []) in io_return _ (s0, r)
-
-sub_effect PURE ~> IOStHistwp = lift_pure_iosthistwp
-
 // given a initial state, returns that state modified and a result
-// let iost_update (event:io_event) : iost unit =
-//   (fun s0 -> io_return _ (event :: s0, ()))
-// let iost_get () : iost events_trace =
-//   (fun s0 -> io_return _ (s0, s0))
+let iost_update (event:io_event) : iost unit =
+  (fun s0 -> io_return _ (event :: s0, ()))
+let iost_get () : iost events_trace =
+  (fun s0 -> io_return _ (s0, s0))
+
+let update (event:io_event) : IOStHistwp unit 
+  (fun s0 p -> p (Inl ((event :: s0), ())) []) by (compute ()) =
+  IOStHistwp?.reflect (
+    fun s0 -> io_return _ (event :: s0, ()))
+
+let get () : IOStHistwp events_trace
+  (fun s0 p -> p (Inl (s0, s0)) []) = 
+  IOStHistwp?.reflect (
+    fun s0 -> io_return _ (s0, s0))
+
+let raise #a (err:exn) : IOStHistwp a
+  (fun s0 p -> p (Inr err) []) =
+  IOStHistwp?.reflect (
+    fun s0 -> io_throw _ err)
 
 effect IOStHist
   (a:Type)
@@ -155,16 +119,12 @@ effect IOStHist
   IOStHistwp a (fun (s0:events_trace) (p:iosthist_post a) ->
     pre s0 /\ (forall res le. post s0 res le ==>  p res le))
 
-
 exception Contract_failure
 
-let get () : IOStHistwp events_trace (fun s0 p -> p (Inl (s0, s0)) []) =
-  IOStHistwp?.reflect(fun _ s0 -> io_return (events_trace * events_trace) (s0, s0))
-  
-let throw (err:exn) : IOStHistwp events_trace (fun s0 p -> p (Inr err) []) =
-  IOStHistwp?.reflect(fun _ s0 -> io_throw _ err)
+let lift_io_iost #a (m:io a) : iost a =
+  fun s0 ->
+    io_bind a (events_trace * a) m (fun x -> io_return (events_trace * a) (s0, x))
 
-// type iost a = events_trace -> io (events_trace * a)
   
 // DEFINE THE PRIMITIVES
 type check_type = (state:events_trace) -> (action:action_type) -> Tot bool
@@ -179,60 +139,49 @@ let default_check (state:events_trace) (action:action_type) =
 unfold
 let apply_changes (old_state local_trace:events_trace) = (List.rev local_trace) @ old_state
 
-unfold let convert_event_to_action (event:io_event) : action_type =
-  match event with
-  | EOpenfile args _ -> (| Openfile, args |)
-  | ERead args _ -> (| Read, args |)
-  | EClose args _ -> (| Close, args |)
-
-
 let rec fold_left (check : (events_trace -> action_type -> bool)) (h : events_trace) : bool =
   match h with
   | [] -> true
-  | h  ::  t ->
+  | h  ::  t -> 
        let action = convert_event_to_action h in
-       if check t action then
+       if check t action then 
          fold_left (check) t
        else false
 
-let some_wp (cmd : io_cmds) (argz: args cmd) = (fun s0 p -> 
-  // precondition
-  (default_check s0 (| cmd, argz |)) /\
-  (forall (result:maybe (events_trace * (res cmd))) local_trace.
-      (match result with
-      | Inl v -> let (s1, r) = v in (
-          local_trace == [convert_call_to_event cmd argz (Inl r)] /\
-          s1 == (apply_changes s0 local_trace))
-      | Inr _ -> True) ==>  p result local_trace))
-
-let ioo_bind #a #b = io_bind a b
+let bind #a #b = iost_bind a b
 
 let static_cmd
   (cmd : io_cmds)
   (argz : args cmd) :
-  IOStHistwp (res cmd) (some_wp cmd argz)
+  IOStHist (res cmd)
+    (requires (fun s0 -> default_check s0 (| cmd, argz |)))
+    (ensures (fun s0 (result:maybe (events_trace * (res cmd))) local_trace ->
+      (match result with
+      | Inl v -> let (s1, r) = v in (
+          local_trace == [convert_call_to_event cmd argz (Inl r)] /\
+          s1 == (apply_changes s0 local_trace)
+      )
+      | Inr _ -> True)))
   by (
-    let cmd' = match List.Tot.nth (cur_binders ()) 0 with
-    | Some x -> x | None -> fail "verification condition changed" in
-    destruct (binder_to_term cmd');
+    let cm' = match List.Tot.nth (cur_binders ()) 0 with
+    | Some x -> x | None -> fail "adsF" in
+    destruct (binder_to_term cm');
     iterAll(fun () ->
       ignore(intro ());
       rewrite_eqs_from_context ();
       compute ()
     )
-  ) =
-  IOStHistwp?.reflect(fun p (s0:events_trace) -> 
-      ((io_all cmd argz) `ioo_bind` 
-      (fun r -> io_return _ (s0, r))) `ioo_bind`
-      (fun (s0, rez) -> io_return _ ((convert_call_to_event cmd argz (Inl rez)) :: s0, rez))
-  )
+  )=
+  let rez = IOStHist?.reflect(lift_io_iost #(res cmd) (io_all cmd argz)) in 
+  update (convert_call_to_event cmd argz (Inl rez));
+  rez
 
 let pi_static_cmd
   (cmd : io_cmds)
   (pi_check : check_type)
   (argz : args cmd) :
   IOStHist (res cmd)
-    (requires (fun s0 ->
+    (requires (fun s0 -> 
       default_check s0 (| cmd, argz |) &&
       pi_check s0 (| cmd, argz |)))
     (ensures (fun s0 (result:maybe (events_trace * (res cmd))) local_trace ->
@@ -245,7 +194,7 @@ let pi_static_cmd
 
 exception GIO_default_check_failed
 exception GIO_pi_check_failed
-
+  
 let mixed_cmd
   (cmd : io_cmds)
   (pi_check : check_type)
@@ -258,11 +207,11 @@ let mixed_cmd
           local_trace == [convert_call_to_event cmd argz (Inl r)] /\
           s1 == (apply_changes s0 local_trace))
       | Inr _ -> True))) =
-  let s0 = get () in
+  let s0 = IOStHist?.reflect (iost_get ()) in
   let action = (| cmd, argz |) in
   match pi_check s0 action with
   | true -> pi_static_cmd cmd pi_check argz
-  | false -> throw GIO_pi_check_failed
+  | false -> IOStHist?.reflect(iost_throw (res cmd) GIO_pi_check_failed)
 
 let dynamic_cmd
   (cmd : io_cmds)
@@ -275,18 +224,18 @@ let dynamic_cmd
       | Inl v -> let (s1, r) = v in (
           local_trace == [convert_call_to_event cmd argz (Inl r)] /\
           s1 == (apply_changes s0 local_trace))
-      | Inr _ -> True))) =
+      | Inr _ -> True))) by (explode (); bump_nth 2; dump "h") =
   let s0 = get () in
   let action = (| cmd, argz |) in
   match default_check s0 action with
-  | true -> mixed_cmd cmd pi_check argz
-  | false -> throw GIO_default_check_failed
+  | true -> mixed_cmd cmd pi_check argz 
+  | false -> raise GIO_default_check_failed
 
 effect GIO
   (a:Type)
   (pi_check : check_type) =
-  IOStHist a
-    (requires (fun s0 ->
+  IOStHist a 
+    (requires (fun s0 -> 
       fold_left default_check s0 &&
       fold_left pi_check s0))
     (ensures (fun s0 (result) local_trace ->
@@ -297,27 +246,4 @@ effect GIO
           fold_left (pi_check) s1)
       | Inr _ -> True)))
 
-val to_runtime_check : (#t1:Type) -> (#t2:Type) -> pre:(t1->events_trace->Type0) -> post:(t1->events_trace->maybe (events_trace * t2)->events_trace->Type0) ->
-  ((x:t1) -> IOStHist t2 (pre x) (post x)) -> 
-  Tot ((x:t1) -> IOStHist t2 (fun _ -> True) (fun s0 result le ->
-    post x s0 result le /\
-    // this is trying to enforce the pre condition, but this is not enough
-    // I suppose a match on result is needed and checked if it was a contract_failure or not
-    (match result with
-    | Inr Contract_failure -> le == []
-    | _ -> pre x s0)))
-
-
-
-val enforce : (#t1:Type) -> (#t2:Type) -> pre:(t1->events_trace->Type0) -> post:(t1->events_trace->maybe (events_trace * t2)->events_trace->Type0) ->
-  (pi_check:check_type) -> ((x:t1) -> IOStHist t2 (pre x) (post x)) -> 
-  Tot ((x:t1) -> IOStHist t2 (pre x) (fun s0 result le ->
-    post x s0 result le /\
-    (match result with
-    | Inl v -> let (s1, r) = v in (
-        s1 == (apply_changes s0 le) /\
-        // this one does not make sense
-        fold_left (pi_check) s1)
-    | Inr _ -> True)))
-    
 
