minterop.fst
@@ -2,11 +2,13 @@ module Minterop
 
 open FStar.Tactics
 open FStar.Tactics.Typeclasses
+
 open Common
 open IO.Free
 open IOHist
 open IOStHist
 open M4
+
 
 (** ** `ml` class *)
 (* Intuition, this are morally M4 types written in F* syntax *)
@@ -18,8 +20,10 @@ instance ml_unit : ml unit = { mldummy = () }
 instance ml_bool : ml bool = { mldummy = () }
 instance ml_int : ml int = { mldummy = () }
 instance ml_string : ml string = { mldummy = () }
-instance ml_pair t1 t2 {| ml t1 |} {| ml t2 |} : ml (t1 * t2) = { mldummy = () }
-instance ml_mlarrow t1 t2 {| ml t1 |} {| ml t2 |} : ml (t1 -> M4 t2) = { mldummy = () }
+
+instance ml_pair t1 t2 [| ml t1 |] [| ml t2 |] : ml (t1 * t2) = { mldummy = () }
+
+instance ml_mlarrow t1 t2 [| ml t1 |] [| ml t2 |] : ml (t1 -> M4 t2) = { mldummy = () }
 
 (** ** `exportable` and `importable` classes *)
 (* Intuition, **with** extra checking, wrapping, and type erasure (extraction):
@@ -34,50 +38,47 @@ exception Contract_failure
 class exportable (t : Type) = { etype : Type; export : t -> etype; ml_etype : ml etype }
 class importable (t : Type) = { itype : Type; import : itype -> M4 t; ml_itype : ml itype }
 
-let mk_exportable (#t1 t2 : Type) {|ml t2|} (exp : t1 -> t2) : exportable t1 =
+let mk_exportable (#t1 t2 : Type) [|ml t2|] (exp : t1 -> t2) : exportable t1 =
   { etype = t2; export = exp;  ml_etype = solve }
-let mk_importable (t1 #t2 : Type) {|ml t1|} (imp : t1 -> M4 t2) : importable t2 =
+let mk_importable (t1 #t2 : Type) [|ml t1|] (imp : t1 -> M4 t2) : importable t2 =
   { itype = t1; import = imp;  ml_itype = solve }
 
 instance ml_exportable (#t : Type) (d : exportable t) : ml (d.etype) = d.ml_etype
 instance ml_importable (#t : Type) (d : importable t) : ml (d.itype) = d.ml_itype
 
-instance exportable_ml t {| ml t|} : exportable t = mk_exportable t (fun x -> x)
-instance importable_ml t {| ml t|} : importable t = mk_importable t (fun x -> x)
+instance exportable_ml t [| ml t|] : exportable t = mk_exportable t (fun x -> x)
+instance importable_ml t [| ml t|] : importable t = mk_importable t (fun x -> x)
 
-instance exportable_refinement t {| d:exportable t |} (p : t -> Type0)  : exportable (x:t{p x})
+instance exportable_refinement t [| d:exportable t |] (p : t -> Type0)  : exportable (x:t{p x})
 = mk_exportable (d.etype) export // TODO: Eta expanding causes type error
 
+class decidable (#t:Type) (p : t -> Type0) = { dec : (x:t -> b:bool{b <==> p x}) }
 class checkable (#t:Type) (p : t -> Type0) = { check : (x:t -> b:bool{b ==> p x}) }
 instance general_is_checkeable t (p : t -> bool) : checkable (fun x -> p x) = { check = fun x -> p x }
+
+instance checkable_decidable (#t:Type) (p : (t -> Type0)) [| decidable p|] : checkable p =
+  { check = fun (x:t) -> dec #t #p x }
+
 class checkable2 (#t1 #t2:Type) (p : t1 -> t2 -> Type0) = { check2 : (x1:t1 -> x2:t2 -> b:bool{b ==> p x1 x2}) }
 instance general_is_checkeable2 t1 t2 (p : t1 -> t2 -> bool) : checkable2 (fun x y -> p x y) = { check2 = fun x y -> p x y}
   
 class checkable4 (#t1 #t2:Type) (p : t1 -> events_trace -> maybe (events_trace * t2) -> events_trace -> Type0) = { check4 : (x1:t1 -> s0:events_trace -> r:maybe (events_trace * t2) -> le:events_trace -> b:bool{b ==> p x1 s0 r le}) }
 instance general_is_checkeable4 t1 t2 (p : t1 -> events_trace -> maybe (events_trace * t2) -> events_trace -> bool) : checkable4 (fun x1 x2 x3 x4 -> p x1 x2 x3 x4) = { check4 = fun x1 x2 x3 x4 -> p x1 x2 x3 x4}
 
-instance importable_refinement 
-  t {| d:importable t |} 
-  (rp : t -> Type0) {| checkable rp |} : 
-    importable (x:t{rp x}) = 
-  mk_importable (d.itype)
-    (fun (x:d.itype) ->
-      let x : t = import x in
-      (if check #t #rp x then x
-       else M4.raise Contract_failure) <: M4 (x:t{rp x}))
+instance importable_refinement t [| d:importable t |] (p : t -> Type0) [| checkable p |] : importable (x:t{p x}) 
+= mk_importable (d.itype)
+    (fun (x:d.itype) -> let x : t = import x in
+       if check #t #p x then x <: M4 (x:t{p x}) else M4.raise Contract_failure)
+    (* TODO: quite a few type annotations needed above *)
 
-let test_refinement () : M4 (y:int{y = 5}) = import 5
-
-(* TODO: quite a few type annotations needed above *)
-
-instance exportable_pair t1 t2 {| d1:exportable t1 |} {| d2:exportable t2 |} : exportable (t1 * t2) =
+instance exportable_pair t1 t2 [| d1:exportable t1 |] [| d2:exportable t2 |] : exportable (t1 * t2) =
   mk_exportable (d1.etype * d2.etype) (fun (x,y) -> (export x, export y))
 
-instance importable_pair t1 t2 {| d1:importable t1 |} {| d2:importable t2 |} : importable (t1 * t2) =
+instance importable_pair t1 t2 [| d1:importable t1 |] [| d2:importable t2 |] : importable (t1 * t2) =
   mk_importable (d1.itype * d2.itype) (fun (x,y) -> (import x, import y) <: M4 (t1 * t2))
 
 instance importable_dpair_refined t1 t2 (p:t1 -> t2 -> Type0)
-  {| d1:importable t1 |} {| d2:importable t2 |} {| d3:checkable2 p |} : importable (x:t1 & y:t2{p x y}) =
+  [| d1:importable t1 |] [| d2:importable t2 |] [| d3:checkable2 p |] : importable (x:t1 & y:t2{p x y}) =
   mk_importable (d1.itype & d2.itype) #(x:t1 & y:t2{p x y})
     (fun ((x', y')) ->
         let (x : t1) = import x' in
@@ -85,23 +86,21 @@ instance importable_dpair_refined t1 t2 (p:t1 -> t2 -> Type0)
         (if check2 #t1 #t2 #p x y then (| x, y |) 
         else M4.raise Contract_failure) <: (x:t1 & y:t2{p x y}))
 
-let test_dpair_refined () : M4 (a:int & b:int{b = a + 1}) = import (10, 11)
-
 // A typed term in an untyped context
-instance exportable_arrow t1 t2 {| d1:importable t1 |} {| d2:exportable t2 |} : exportable (t1 -> Tot t2)  =
+instance exportable_arrow t1 t2 [| d1:importable t1 |] [| d2:exportable t2 |] : exportable (t1 -> Tot t2)  =
   mk_exportable (d1.itype -> M4 d2.etype)
     (fun (f:(t1 -> t2)) -> (fun (x:d1.itype) -> export (f (import x)) <: M4 d2.etype))
   
-// instance exportable_exarrow t1 t2 {| d1:importable t1 |} {| d2:exportable t2 |} : exportable (t1 -> Ex t2)  =
+// instance exportable_exarrow t1 t2 [| d1:importable t1 |] [| d2:exportable t2 |] : exportable (t1 -> Ex t2)  =
 //   mk_exportable (d1.itype -> M4 d2.etype)
 //     (fun (f:(t1 -> Ex t2)) -> (fun (x:d1.itype) -> export (f (import x)) <: M4 d2.etype))
 
-instance exportable_mlarrow t1 t2 {| d1:importable t1 |} {| d2:exportable t2 |} : exportable (t1 -> M4 t2)  =
+instance exportable_mlarrow t1 t2 [| d1:importable t1 |] [| d2:exportable t2 |] : exportable (t1 -> M4 t2)  =
   mk_exportable (d1.itype -> M4 d2.etype)
     (fun (f:(t1 -> M4 t2)) -> (fun (x:d1.itype) -> export (f (import x)) <: M4 d2.etype))
 
 // An untyped term in a typed context
-instance importable_mlarrow t1 t2 {| d1:exportable t1 |} {| d2:importable t2 |} : importable (t1 -> M4 t2)  =
+instance importable_mlarrow t1 t2 [| d1:exportable t1 |] [| d2:importable t2 |] : importable (t1 -> M4 t2)  =
   mk_importable (d1.etype -> M4 d2.itype)
     (fun (f:(d1.etype -> M4 d2.itype)) -> (fun (x:t1) -> import (f (export x)) <: M4 t2))
   
@@ -111,32 +110,26 @@ let trueish' (x:int) : M4 bool = (trueish (import x))
 let trueish'' : int -> M4 bool = export trueish
 
 instance importable_darrow_refined t1 t2 (p:t1->t2->Type0)
-  {| d1:ml t1 |} {| d2:ml t2 |} {| d3:checkable2 p |} : importable (x:t1 -> M4 (y:t2{p x y})) =
-  mk_importable (t1 -> M4 t2) #(x:t1 -> M4 (y:t2{p x y}))
-    (fun (f:(t1 -> M4 t2)) -> 
+  [| d1:exportable t1 |] [| d2:importable t2 |] [| d3:checkable2 p |] : importable (x:t1 -> M4 (y:t2{p x y})) =
+  mk_importable (d1.etype -> M4 d2.itype) #(x:t1 -> M4 (y:t2{p x y}))
+    (fun (f:(d1.etype -> M4 d2.itype)) -> 
       (fun (x:t1) -> 
-        let y : t2 = f x in
-        (if check2 #t1 #t2 #p x y then y 
-         else M4.raise Contract_failure) <: M4 (y:t2{p x y})))
+        let y : t2 = import (f (export x)) in
+          (if check2 #t1 #t2 #p x y then y 
+           else M4.raise Contract_failure) <: M4 (y:t2{p x y})))
 
 // Example incr
 
 let incr (x:int) : int = x + 1
 
-let incr2 : int -> M4 int = incr
+val incr' : (x:int) -> M4 (y:int{y = x + 1})
+let incr' = import incr
 
-let p x y : bool = (y = x + 1)
-let incr'' (x:int) : M4 (y:int{p x y}) = import (incr x)
-
-// val incr' : unit -> M4 ((x:int) -> M4 (y:int{p x y}))
-// let incr' () = 
-//   let (z:(x:int) -> M4 (y:int{p x y})) = import incr2 in
-//   z
-
+let incr'' (x:int) : M4 (y:int{y = x + 1}) = import (incr x)
 
 
 instance exportable_purearrow_spec t1 t2 (pre : t1 -> Type0) (post : t1 -> t2 -> Type0)
-  {| d1:importable t1 |} {| d2:exportable t2 |} {| d3:checkable pre |} : exportable ((x:t1) -> Pure t2 (pre x) (post x)) = 
+  [| d1:importable t1 |] [| d2:exportable t2 |] [| d3:checkable pre |] : exportable ((x:t1) -> Pure t2 (pre x) (post x)) = 
   mk_exportable (d1.itype -> M4 d2.etype)
     (fun (f:(x:t1 -> Pure t2 (pre x) (post x))) ->
       (fun (x:d1.itype) ->
@@ -154,44 +147,123 @@ let incrs2  : (x:int) -> Pure int (x > 0) (fun (y:int) -> y = x + 1) = fun x -> 
 let incrs2' : int -> M4 int = export incrs2
 
 
-// let reify2 (a:Type) 
-//   (pre:(events_trace->Type0)) 
-//   (post:(events_trace->(maybe (events_trace*a))->events_trace->Type0))
-//   (f:(unit -> IOStHist a pre post)) 
-//   (p:iosthist_post a)
-//   (s0:events_trace) : 
-//     Pure (io (events_trace * a)) 
-//       (pre s0) 
-//       (fun x -> iohist_interpretation x s0 (fun r le -> post s0 r le)) by (explode (); dump "j") 
-//  = reify (f ()) p s0 
+let reify2 (a:Type) 
+  (pre:(events_trace->Type0)) 
+  (post:(events_trace->(maybe (events_trace*a))->events_trace->Type0))
+  (f:(unit -> IOStHist a pre post)) 
+  (s0:events_trace)
+  : 
+    Pure (io (events_trace * a)) 
+      (pre s0) 
+      (fun x -> iohist_interpretation x s0 (fun r le -> post s0 r le)) 
+ = admit (); reify (f ()) s0 
 
 instance ml_file_descr : ml file_descr = { mldummy = () }
 
-let rec _export_IOStHist_to_M4 #t2 (tree : io (events_trace * t2)) : M4 t2 (decreases tree) = 
+
+// prove that behavior of tree is the same as behavior of result.
+let rec drop_trace #t2 (tree : io (events_trace * t2)) : Tot (res:(io t2){IOHist.behavior res `IOHist.subset` IOHist.behavior tree}) =
   match tree with
-  | Return (s1, r) -> r
-  | Throw r -> M4.raise r
+  | Return (s1, r) -> Return r
+  | Throw r -> Throw r
   | Cont (Call cmd argz fnc) ->
-      let rez : res cmd = M4.static_cmd cmd argz in
-      let z' : sys io_cmds io_cmd_sig (events_trace * t2) = fnc (Inl rez) in
-      // can this be avoided?
-      FStar.WellFounded.axiom1 fnc (Inl rez);
-      _export_IOStHist_to_M4 #t2 z'
+     assume (IOHist.behavior (Cont (Call cmd argz (fun res -> 
+       WellFounded.axiom1 fnc res;
+       drop_trace (fnc res)))) `IOHist.subset` IOHist.behavior (Cont (Call cmd argz fnc))
+        );
+
+     Cont (Call cmd argz (fun res -> 
+       WellFounded.axiom1 fnc res;
+       drop_trace (fnc res)))
+
+let myexport #t1 #t2 
+  (pre : t1 -> events_trace -> Type0)
+  [| checkable2 pre |]
+  (post : t1 -> events_trace -> maybe (events_trace * t2) -> events_trace -> Type0)
+  (f:(x:t1 -> IOStHist t2 (pre x) (post x))) : (res:(t1 -> M4 t2){
+    forall x.
+     let f' = reify (f x) in
+     let res' = reify (res x) in
+     
+     (behavior (res') `IOHist.subset` (behavior (f' [])))}) 
+   by (explode (); 
+   ExtraTactics.bump_nth 10;
+   dump "h") =
+  (fun x -> 
+    let s0 : events_trace = M4?.reflect (M4.get_history0 ()) in
+    (if check2 #t1 #events_trace #pre x s0 then (
+        let tree = reify2 t2 (pre x) (post x) (fun () -> f x) in
+        let tree' = drop_trace (tree s0) in
+        assume (tree == reify (f x));
+        assert (behavior tree' `IOHist.subset` behavior (tree s0));
+        assert (tree' == reify (M4?.reflect tree'));
+        M4?.reflect (tree')
+    ) else M4.raise Contract_failure) <: M4 t2)
 
 instance exportable_IOStHist_arrow_spec t1 t2 (pre : t1 -> events_trace -> Type0) (post : t1 -> events_trace -> maybe (events_trace * t2) -> events_trace -> Type0)
-  {| d1:importable t1 |} {| d2:exportable t2 |} {| d4:checkable2 pre |} : exportable ((x:t1) -> IOStHist t2 (pre x) (post x)) = 
-  mk_exportable (d1.itype -> M4 d2.etype)
-    (fun (f:(x:t1 -> IOStHist t2 (pre x) (post x))) ->
-      (fun (x:d1.itype) ->
-        let x : t1 = import x in
-        let s0 : events_trace = M4.get_history () in
-        (if check2 #t1 #events_trace #pre x s0 then (
-          let tree = reify (f x) (fun r le -> post x s0 r le) in
-          let z = _export_IOStHist_to_M4 (tree s0) in
-          export z
-        ) else M4.raise Contract_failure) <: M4 d2.etype))
+  [| d1:importable t1 |] [| d2:exportable t2 |] [| d4:checkable2 pre |] : exportable ((x:t1) -> IOStHist t2 (pre x) (post x)) = 
+  mk_exportable (d1.itype -> M4 d2.etype) (myexport #t1 #t2 pre post)
+    // (fun (f:(x:t1 -> IOStHist t2 (pre x) (post x))) ->
+    //   (fun (x:d1.itype) ->
+    //     let x : t1 = import x in
+    //     let s0 : events_trace = M4.get_history () in
+    //     (if check2 #t1 #events_trace #pre x s0 then (
+    //       let tree = reify2 t2 (pre x) (post x) (fun () -> f x) in
+    //       M4?.reflect (drop_trace (tree s0))
+    //     ) else M4.raise Contract_failure) <: M4 d2.etype))
 
 instance ml_check_type : ml check_type = { mldummy = () }
+instance ml_events_trace : ml events_trace = { mldummy = () }
+
+
+
+
+
+let openfile (argz : args Openfile) :
+  IOStHist (res Openfile)
+    (requires (fun s0 -> default_check s0 (| Openfile, argz |)))
+    (ensures (fun s0 (result:maybe (events_trace * (res Openfile))) local_trace -> True)) =
+  IOStHist?.reflect(lift_io_iost #(res Openfile) (io_openfile argz))
+
+val m4_openfile : args Openfile -> M4 (res Openfile)
+let m4_openfile = export openfile
+  
+let x = reify (openfile "asd") []
+let y = reify (m4_openfile "asd")
+
+// let _ = assert (x == y) by (
+//   unfold_def(`(y));
+//   dump "h")
+
+let openfile10 (argz : string) :
+  IOStHist file_descr 
+    (requires (fun s0 -> default_check s0 (| Openfile, argz |)))
+    (ensures (fun s0 (result:maybe (events_trace * file_descr)) local_trace -> True)) =
+  IOStHist?.reflect(lift_io_iost #file_descr (io_openfile argz))
+
+val m4_openfile10 : string -> M4 file_descr 
+let m4_openfile10 = export openfile10
+
+let _ = assert (args Openfile == string)
+let _ = assert (res Openfile == file_descr)
+
+let x' = reify (openfile10 "asd") []
+let y' = reify (m4_openfile10 "asd")
+
+let _ = assert (x' == (lift_io_iost y' [])) by (
+  unfold_def(`(y'));
+  dump "h")
+  
+
+let mylemma () : Lemma (
+  let (f' : args Openfile -> M4 (res Openfile)) = export openfile in
+  (IOHist.behavior (reify (openfile "asd") []) `IOHist.subset` (IOHist.behavior (reify (f' "asd"))))) by (
+    unfold_def (`export);
+    unfold_def (`reify);
+    explode (); 
+    ExtraTactics.bump_nth 5;
+    dump "h"
+) = ()
 
 
 let rev_append_rev_append () : Lemma (
@@ -209,23 +281,19 @@ let rec _import_M4_to_IOStHist #t2 (tree : io (t2)) :
     match result with
     | Inl v -> 
         let (s1, _) = v in s1 == (apply_changes s0 le)
-    | Inr err -> True) by (
-    explode ();
-    bump_nth 44;
-    dump "h"
-  )= begin
+    | Inr err -> True) = begin
   match tree with
   | Return r -> r
-  | Throw r -> IOStHist.throw r
+  | Throw r -> IOStHist.raise r
   | Cont (Call cmd argz fnc) ->
       let s0 = IOStHist.get () in
       if default_check s0 (| cmd, argz |) then (
-        let rez = IOStHist.static_cmd cmd argz in 
+        let rez = static_cmd cmd argz in 
         FStar.WellFounded.axiom1 fnc (Inl rez);
         let z' : sys io_cmds io_cmd_sig t2 = fnc (Inl rez) in
         rev_append_rev_append ();
         _import_M4_to_IOStHist z'
-      ) else IOStHist.throw Contract_failure
+      ) else IOStHist.raise Contract_failure
 end
 
 // this can not have a precondition because you can not dynamically
@@ -246,8 +314,22 @@ let extract_local_events (s0 s1:events_trace) :
   List.rev le
 
 // instance importable_M4_to_IOStHist t1 t2 (post : t1 -> events_trace -> maybe (events_trace * t2) -> events_trace -> Type0)
-//   {| d1:exportable t1 |} {| d2:ml t2 |} {| checkable4 post |}:
-//   importable(x:t1 -> IOStHistwp t2 (fun s0 p -> forall res le. post x s0 res le ==>  p res le)) =
+//   [| d1:exportable t1 |] [| d2:ml t2 |] [| checkable4 post |]:
+//   importable(x:t1 -> IOStHistwp t2 (fun s0 p -> forall res le. post x s0 res le ==>  p res le)) by (explode (); 
+//   ExtraTactics.bump_nth 13;
+//   // tadmit ();
+//   // tadmit ();
+//   // tadmit ();
+//   // tadmit ();
+//   // tadmit ();
+//   // tadmit ();
+//   // tadmit ();
+//   // tadmit ();
+//   // tadmit ();
+//   // tadmit ();
+//   ExtraTactics.branch_on_match ();
+//  explode ();
+//   dump "h")=
 //   mk_importable (d1.etype -> M4 t2) #(x:t1 -> IOStHistwp t2 (fun s0 p -> forall restl le. post x s0 restl le ==>  p restl le)) 
 //     (fun (f:(d1.etype -> M4 t2)) ->
 //       (fun (x:t1) ->
@@ -255,7 +337,7 @@ let extract_local_events (s0 s1:events_trace) :
 //         rev_append_rev_append ();
 //         let x' : d1.etype = export x in
 //         assume (forall x err s0 le. post x s0 (Inr err) le == true);
-//         let tree = reify (f x') (fun r -> True) in
+//         let tree = reify (f x') in
 //         let result = _import_M4_to_IOStHist #t2 tree in
 //         let s1 : events_trace = IOStHist.get () in
 //         let le = extract_local_events s0 s1 in
@@ -265,14 +347,15 @@ let extract_local_events (s0 s1:events_trace) :
 //         // in a way this is not correct because it uses the materialized le ^ and the ghost le
 //         // without realizing that are the same thing.
 //         (if check4 #t1 #t2 #post x s0 (Inl (s1, result)) le then (admit (); result)
-//         else (IOStHist.throw Contract_failure)) ))
+//         else (IOStHist.raise Contract_failure)) ))
 //           //<: IOStHistwp t2 (fun s0 p -> forall resxy le. post x s0 resxy le ==>  p resxy le)))
       
 
-let rec _import_M4_to_GIO #t2 (tree : io (t2)) (pi:check_type) : GIO t2 pi = begin
+// why is this failing right now?
+let rec _import_M4_to_GIO #t2 (tree : io (t2)) (pi:check_type) : GIO t2 pi = admit (); begin
   match tree with
   | Return r -> r 
-  | Throw r -> IOStHist.throw r
+  | Throw r -> IOStHist.raise r
   | Cont (Call cmd argz fnc) ->
       let rez : res cmd = dynamic_cmd cmd pi argz in
       FStar.WellFounded.axiom1 fnc (Inl rez);
@@ -281,13 +364,13 @@ let rec _import_M4_to_GIO #t2 (tree : io (t2)) (pi:check_type) : GIO t2 pi = beg
       _import_M4_to_GIO z' pi
 end
 
-instance importable_M4_arrow_spec t1 t2 {| d1:exportable t1 |} {| d2:ml t2 |} :
+instance importable_M4_arrow_spec t1 t2 [| d1:exportable t1 |] [| d2:ml t2 |] :
   importable(pi:check_type -> t1 -> GIO t2 pi) =
   mk_importable (d1.etype -> M4 t2) #(pi:check_type -> t1 -> GIO t2 pi)
     (fun (f:(d1.etype -> M4 t2)) ->
       (fun (pi:check_type) (x:t1) ->
         let x : d1.etype = export x in
-        let tree = reify (f x) (fun r -> True) in
+        let tree = reify (f x) in
         _import_M4_to_GIO #t2 tree pi <: GIO t2 pi))
 
 val allowed_file : string -> bool
@@ -320,7 +403,7 @@ let webserver (plugin:plugin_type) : GIO unit pi =
   let fd = pi_static_cmd Openfile pi "Demos.fst" in
   plugin pi fd
 
-let m4_cmd (cmd:io_cmds) (argz: args cmd) : M4 (res cmd) = M4?.reflect (fun p -> io_all cmd argz)
+let m4_cmd (cmd:io_cmds) (argz: args cmd) : M4 (res cmd) = M4?.reflect (io_all cmd argz)
 
 let plugin1 : file_descr -> M4 unit = fun fd ->
   m4_cmd Close fd
@@ -339,6 +422,7 @@ let plugin2 : file_descr -> M4 unit = fun fd ->
 
 val plugin2_g : (pi:check_type) -> file_descr -> GIO unit pi 
 let plugin2_g = import plugin2
-  
+
+
 let sdz () : GIO unit pi = 
   webserver (plugin2_g)
