test.fst
@@ -1,0 +1,18 @@
+
+
+let openfile10
+  (argz : string) :
+  IOStHist file_descr 
+    (requires (fun s0 -> default_check s0 (| Openfile, argz |)))
+    (ensures (fun s0 (result:maybe (events_trace * file_descr)) local_trace -> True)) =
+  IOStHist?.reflect(lift_io_iost #file_descr (io_openfile argz))
+
+val m4_openfile10 : string -> M4 file_descr 
+let m4_openfile10 = export openfile10
+
+let x = reify (openfile10 "asd") []
+let y = reify (m4_openfile10 "asd")
+let _ = assert (x == y) by (
+  unfold_def(`y);
+  dump "h")
+  
